feat: remove `Finite` conditions from iterator consumers relying on a new fixpoint combinator (#11038)
This PR introduces a new fixpoint combinator,
`WellFounded.extrinsicFix`. A termination proof, if provided at all, can
be given extrinsically, i.e., looking at the term from the outside, and
is only required if one intends to formally verify the behavior of the
fixpoint. The new combinator is then applied to the iterator API.
Consumers such as `toList` or `ForIn` no longer require a proof that the
underlying iterator is finite. If one wants to ensure the termination of
them intrinsically, there are strictly terminating variants available
as, for example, `it.ensureTermination.toList` instead of `it.toList`.

src/Init/Data/Iterators/Consumers/Monadic/Loop.lean
@@ -8,6 +8,8 @@ module
 prelude
 public import Init.Data.Iterators.Consumers.Monadic.Partial
 public import Init.Data.Iterators.Internal.LawfulMonadLiftFunction
+public import Init.WFExtrinsicFix
+public import Init.Data.Iterators.Consumers.Monadic.Total
 
 public section
 
@@ -24,7 +26,7 @@ function in every iteration. Concretely, the following operations are provided:
   be used to apply the monadic effects of the iterator.
 
 Some producers and combinators provide specialized implementations. These are captured by the
-`IteratorLoop` and `IteratorLoopPartial` typeclasses. They should be implemented by all
+`IteratorLoop` type class. They should be implemented by all
 types of iterators. A default implementation is provided. The typeclass `LawfulIteratorLoop`
 asserts that an `IteratorLoop` instance equals the default implementation.
 -/
@@ -57,8 +59,9 @@ def IteratorLoop.WellFounded (α : Type w) (m : Type w → Type w') {β : Type w
 
 /--
 `IteratorLoop α m` provides efficient implementations of loop-based consumers for `α`-based
-iterators. The basis is a `ForIn`-style loop construct with the complication that it can be used
-for infinite iterators, too -- given a proof that the given loop will nevertheless terminate.
+iterators. The basis is a `ForIn`-style loop construct.
+
+Its behavior for well-founded loops is fully characterized by the `LawfulIteratorLoop` type class.
 
 This class is experimental and users of the iterator API should not explicitly depend on it.
 They can, however, assume that consumers that require an instance will work for all iterators
@@ -69,24 +72,9 @@ class IteratorLoop (α : Type w) (m : Type w → Type w') {β : Type w} [Iterato
     (n : Type x → Type x') where
   forIn : ∀ (_liftBind : (γ : Type w) → (δ : Type x) → (γ → n δ) → m γ → n δ) (γ : Type x),
       (plausible_forInStep : β → γ → ForInStep γ → Prop) →
-      IteratorLoop.WellFounded α m plausible_forInStep →
       (it : IterM (α := α) m β) → γ →
       ((b : β) → it.IsPlausibleIndirectOutput b → (c : γ) → n (Subtype (plausible_forInStep b c))) →
       n γ
-
-/--
-`IteratorLoopPartial α m` provides efficient implementations of loop-based consumers for `α`-based
-iterators. The basis is a partial, i.e. potentially nonterminating, `ForIn` instance.
-
-This class is experimental and users of the iterator API should not explicitly depend on it.
-They can, however, assume that consumers that require an instance will work for all iterators
-provided by the standard library.
--/
-class IteratorLoopPartial (α : Type w) (m : Type w → Type w') {β : Type w} [Iterator α m β]
-    (n : Type x → Type x') where
-  forInPartial : ∀ (_liftBind : (γ : Type w) → (δ : Type x) → (γ → n δ) → m γ → n δ) {γ : Type x},
-      (it : IterM (α := α) m β) → γ →
-      ((b : β) → it.IsPlausibleIndirectOutput b → (c : γ) → n (ForInStep γ)) → n γ
 
 end Typeclasses
 
@@ -108,64 +96,54 @@ instance IteratorLoop.WithWF.instWellFoundedRelation
 /--
 This is the loop implementation of the default instance `IteratorLoop.defaultImplementation`.
 -/
-@[specialize, expose]
+@[always_inline, inline, expose]
 def IterM.DefaultConsumers.forIn' {m : Type w → Type w'} {α : Type w} {β : Type w}
     [Iterator α m β]
     {n : Type x → Type x'} [Monad n]
     (lift : ∀ γ δ, (γ → n δ) → m γ → n δ) (γ : Type x)
-    (plausible_forInStep : β → γ → ForInStep γ → Prop)
-    (wf : IteratorLoop.WellFounded α m plausible_forInStep)
+    (PlausibleForInStep : β → γ → ForInStep γ → Prop)
     (it : IterM (α := α) m β) (init : γ)
     (P : β → Prop) (hP : ∀ b, it.IsPlausibleIndirectOutput b → P b)
-    (f : (b : β) → P b → (c : γ) → n (Subtype (plausible_forInStep b c))) : n γ :=
+    (f : (b : β) → P b → (c : γ) → n (Subtype (PlausibleForInStep b c))) : n γ :=
+  haveI : Nonempty γ := ⟨init⟩
+  WellFounded.extrinsicFix₃ (C₃ := fun _ _ _ => n γ) (InvImage (IteratorLoop.rel α m PlausibleForInStep) (fun x => (x.1, x.2.1)))
+    (fun it acc (hP : ∀ b, it.IsPlausibleIndirectOutput b → P b) recur => (lift _ _ · it.step) fun s => do
+      match s.inflate with
+      | .yield it' out h =>
+        match ← f out (hP out <| .direct ⟨_, h⟩) acc with
+        | ⟨.yield c, h'⟩ => recur it' c (fun _ h' => hP _ <| .indirect ⟨_, rfl, h⟩ h') (Or.inl ⟨out, ‹_›, ‹_›⟩)
+        | ⟨.done c, h⟩ => return c
+      | .skip it' h => recur it' acc (fun _ h' => hP _ <| .indirect ⟨_, rfl, h⟩ h') (Or.inr ⟨‹_›, rfl⟩)
+      | .done _ => return acc) it init hP
+
+/--
+This is the loop implementation of the default instance `IteratorLoop.defaultImplementation`.
+-/
+@[specialize, expose]
+def IterM.DefaultConsumers.forIn'.wf {m : Type w → Type w'} {α : Type w} {β : Type w}
+    [Iterator α m β] {n : Type x → Type x'} [Monad n]
+    (lift : ∀ γ δ, (γ → n δ) → m γ → n δ) (γ : Type x)
+    (PlausibleForInStep : β → γ → ForInStep γ → Prop)
+    (wf : IteratorLoop.WellFounded α m PlausibleForInStep)
+    (it : IterM (α := α) m β) (init : γ)
+    (P : β → Prop) (hP : ∀ b, it.IsPlausibleIndirectOutput b → P b)
+    (f : (b : β) → P b → (c : γ) → n (Subtype (PlausibleForInStep b c))) : n γ :=
   haveI : WellFounded _ := wf
   (lift _ _ · it.step) fun s =>
     match s.inflate with
     | .yield it' out h => do
       match ← f out (hP _ <| .direct ⟨_, h⟩) init with
       | ⟨.yield c, _⟩ =>
-        IterM.DefaultConsumers.forIn' lift _ plausible_forInStep wf it' c P
+        IterM.DefaultConsumers.forIn'.wf lift _ PlausibleForInStep wf it' c P
           (fun _ h' => hP _ <| .indirect ⟨_, rfl, h⟩ h') f
       | ⟨.done c, _⟩ => return c
     | .skip it' h =>
-      IterM.DefaultConsumers.forIn' lift _ plausible_forInStep wf it' init P
+      IterM.DefaultConsumers.forIn'.wf lift _ PlausibleForInStep wf it' init P
           (fun _ h' => hP _ <| .indirect ⟨_, rfl, h⟩ h') f
     | .done _ => return init
 termination_by IteratorLoop.WithWF.mk it init (hwf := wf)
 decreasing_by
   · exact Or.inl ⟨out, ‹_›, ‹_›⟩
-  · exact Or.inr ⟨‹_›, rfl⟩
-
-theorem IterM.DefaultConsumers.forIn'_eq_forIn' {m : Type w → Type w'} {α : Type w} {β : Type w}
-    [Iterator α m β]
-    {n : Type x → Type x'} [Monad n]
-    {lift : ∀ γ δ, (γ → n δ) → m γ → n δ} {γ : Type x}
-    {Pl : β → γ → ForInStep γ → Prop}
-    {wf : IteratorLoop.WellFounded α m Pl}
-    {it : IterM (α := α) m β} {init : γ}
-    {P : β → Prop} {hP : ∀ b, it.IsPlausibleIndirectOutput b → P b}
-    {Q : β → Prop} {hQ : ∀ b, it.IsPlausibleIndirectOutput b → Q b}
-    {f : (b : β) → P b → (c : γ) → n (Subtype (Pl b c))}
-    {g : (b : β) → Q b → (c : γ) → n (Subtype (Pl b c))}
-    (hfg : ∀ b c, (hPb : P b) → (hQb : Q b) → f b hPb c = g b hQb c) :
-    IterM.DefaultConsumers.forIn' lift γ Pl wf it init P hP f =
-      IterM.DefaultConsumers.forIn' lift γ Pl wf it init Q hQ g := by
-  rw [forIn', forIn']
-  congr; ext step
-  split
-  · congr
-    · apply hfg
-    · ext
-      split
-      · apply IterM.DefaultConsumers.forIn'_eq_forIn'
-        assumption
-      · rfl
-  · apply IterM.DefaultConsumers.forIn'_eq_forIn'
-    assumption
-  · rfl
-termination_by IteratorLoop.WithWF.mk it init (hwf := wf)
-decreasing_by
-  · exact Or.inl ⟨_, ‹_›, ‹_›⟩
   · exact Or.inr ⟨‹_›, rfl⟩
 
 /--
@@ -177,7 +155,7 @@ implementations are possible and should be used instead.
 def IteratorLoop.defaultImplementation {α : Type w} {m : Type w → Type w'} {n : Type x → Type x'}
     [Monad n] [Iterator α m β] :
     IteratorLoop α m n where
-  forIn lift γ Pl wf it init := IterM.DefaultConsumers.forIn' lift γ Pl wf it init _ (fun _ => id)
+  forIn lift γ Pl it init := IterM.DefaultConsumers.forIn' lift γ Pl it init _ (fun _ => id)
 
 /--
 Asserts that a given `IteratorLoop` instance is equal to `IteratorLoop.defaultImplementation`.
@@ -185,49 +163,18 @@ Asserts that a given `IteratorLoop` instance is equal to `IteratorLoop.defaultIm
 -/
 class LawfulIteratorLoop (α : Type w) (m : Type w → Type w') (n : Type x → Type x')
     [Monad m] [Monad n] [Iterator α m β] [i : IteratorLoop α m n] where
-  lawful : ∀ lift [LawfulMonadLiftBindFunction lift], i.forIn lift =
-      IteratorLoop.defaultImplementation.forIn lift
-
-/--
-This is the loop implementation of the default instance `IteratorLoopPartial.defaultImplementation`.
--/
-@[specialize]
-partial def IterM.DefaultConsumers.forInPartial {m : Type w → Type w'} {α : Type w} {β : Type w}
-    [Iterator α m β]
-    {n : Type x → Type x'} [Monad n]
-    (lift : ∀ γ δ, (γ → n δ) → m γ → n δ) (γ : Type x)
-    (it : IterM (α := α) m β) (init : γ)
-    (f : (b : β) → it.IsPlausibleIndirectOutput b → (c : γ) → n (ForInStep γ)) : n γ :=
-  (lift _ _ · it.step) fun s =>
-      match s.inflate with
-      | .yield it' out h => do
-        match ← f out (.direct ⟨_, h⟩) init with
-        | .yield c =>
-          IterM.DefaultConsumers.forInPartial lift _ it' c
-            fun out h' acc => f out (.indirect ⟨_, rfl, h⟩ h') acc
-        | .done c => return c
-      | .skip it' h =>
-        IterM.DefaultConsumers.forInPartial lift _ it' init
-          fun out h' acc => f out (.indirect ⟨_, rfl, h⟩ h') acc
-      | .done _ => return init
-
-/--
-This is the default implementation of the `IteratorLoopPartial` class.
-It simply iterates through the iterator using `IterM.step`. For certain iterators, more efficient
-implementations are possible and should be used instead.
--/
-@[always_inline, inline]
-def IteratorLoopPartial.defaultImplementation {α : Type w} {m : Type w → Type w'}
-    {n : Type x → Type x'} [Monad m] [Monad n] [Iterator α m β] :
-    IteratorLoopPartial α m n where
-  forInPartial lift := IterM.DefaultConsumers.forInPartial lift _
+  lawful lift [LawfulMonadLiftBindFunction lift] γ it init
+      (Pl : β → γ → ForInStep γ → Prop) (wf : IteratorLoop.WellFounded α m Pl)
+      (f : (b : β) → it.IsPlausibleIndirectOutput b → (c : γ) → n (Subtype (Pl b c))) :
+    i.forIn lift γ Pl it init f =
+      IteratorLoop.defaultImplementation.forIn lift γ Pl it init f
 
 instance (α : Type w) (m : Type w → Type w') (n : Type x → Type x')
     [Monad m] [Monad n] [Iterator α m β] [Finite α m] :
     letI : IteratorLoop α m n := .defaultImplementation
-    LawfulIteratorLoop α m n :=
+    LawfulIteratorLoop α m n := by
   letI : IteratorLoop α m n := .defaultImplementation
-  ⟨fun _ => rfl⟩
+  constructor; simp
 
 theorem IteratorLoop.wellFounded_of_finite {m : Type w → Type w'}
     {α β : Type w} {γ : Type x} [Iterator α m β] [Finite α m] :
@@ -247,13 +194,11 @@ This `ForIn'`-style loop construct traverses a finite iterator using an `Iterato
 -/
 @[always_inline, inline]
 def IteratorLoop.finiteForIn' {m : Type w → Type w'} {n : Type x → Type x'}
-    {α : Type w} {β : Type w} [Iterator α m β] [Finite α m] [IteratorLoop α m n] [Monad n]
+    {α : Type w} {β : Type w} [Iterator α m β] [IteratorLoop α m n] [Monad n]
     (lift : ∀ γ δ, (γ → n δ) → m γ → n δ) :
     ForIn' n (IterM (α := α) m β) β ⟨fun it out => it.IsPlausibleIndirectOutput out⟩ where
   forIn' {γ} it init f :=
-    IteratorLoop.forIn (α := α) (m := m) lift γ (fun _ _ _ => True)
-      wellFounded_of_finite
-      it init (fun out h acc => (⟨·, .intro⟩) <$> f out h acc)
+    IteratorLoop.forIn (α := α) (m := m) lift γ (fun _ _ _ => True) it init (return ⟨← f · · ·, trivial⟩)
 
 /--
 A `ForIn'` instance for iterators. Its generic membership relation is not easy to use,
@@ -262,13 +207,13 @@ or future library improvements will make it more comfortable.
 -/
 @[always_inline, inline]
 def IterM.instForIn' {m : Type w → Type w'} {n : Type w → Type w''}
-    {α : Type w} {β : Type w} [Iterator α m β] [Finite α m] [IteratorLoop α m n] [Monad n]
+    {α : Type w} {β : Type w} [Iterator α m β] [IteratorLoop α m n] [Monad n]
     [MonadLiftT m n] :
     ForIn' n (IterM (α := α) m β) β ⟨fun it out => it.IsPlausibleIndirectOutput out⟩ :=
   IteratorLoop.finiteForIn' (fun _ _ f x => monadLift x >>= f)
 
 instance {m : Type w → Type w'} {n : Type w → Type w''}
-    {α : Type w} {β : Type w} [Iterator α m β] [Finite α m] [IteratorLoop α m n]
+    {α : Type w} {β : Type w} [Iterator α m β] [IteratorLoop α m n]
     [MonadLiftT m n] [Monad n] :
     ForIn n (IterM (α := α) m β) β :=
   haveI : ForIn' n (IterM (α := α) m β) β _ := IterM.instForIn'
@@ -276,27 +221,43 @@ instance {m : Type w → Type w'} {n : Type w → Type w''}
 
 @[always_inline, inline]
 def IterM.Partial.instForIn' {m : Type w → Type w'} {n : Type w → Type w''}
-    {α : Type w} {β : Type w} [Iterator α m β] [IteratorLoopPartial α m n] [MonadLiftT m n] [Monad n] :
+    {α : Type w} {β : Type w} [Iterator α m β] [IteratorLoop α m n] [MonadLiftT m n] [Monad n] :
     ForIn' n (IterM.Partial (α := α) m β) β ⟨fun it out => it.it.IsPlausibleIndirectOutput out⟩ where
-  forIn' it init f := IteratorLoopPartial.forInPartial (α := α) (m := m) (n := n)
-      (fun _ _ f x => monadLift x >>= f) it.it init f
+  forIn' it init f :=
+    haveI := @IterM.instForIn'; forIn' it.it init f
+
+@[always_inline, inline]
+def IterM.Total.instForIn' {m : Type w → Type w'} {n : Type w → Type w''}
+    {α : Type w} {β : Type w} [Iterator α m β] [IteratorLoop α m n] [MonadLiftT m n] [Monad n]
+    [Finite α m] :
+    ForIn' n (IterM.Total (α := α) m β) β ⟨fun it out => it.it.IsPlausibleIndirectOutput out⟩ where
+  forIn' it init f := IterM.instForIn'.forIn' it.it init f
 
 instance {m : Type w → Type w'} {n : Type w → Type w''}
-    {α : Type w} {β : Type w} [Iterator α m β] [IteratorLoopPartial α m n] [MonadLiftT m n] [Monad n] :
+    {α : Type w} {β : Type w} [Iterator α m β] [IteratorLoop α m n] [MonadLiftT m n] [Monad n] :
     ForIn n (IterM.Partial (α := α) m β) β :=
   haveI : ForIn' n (IterM.Partial (α := α) m β) β _ := IterM.Partial.instForIn'
   instForInOfForIn'
 
 instance {m : Type w → Type w'} {n : Type w → Type w''}
-    {α : Type w} {β : Type w} [Iterator α m β] [Finite α m] [IteratorLoop α m n] [Monad n]
-    [MonadLiftT m n] :
-    ForM n (IterM (α := α) m β) β where
+    {α : Type w} {β : Type w} [Iterator α m β] [IteratorLoop α m n] [MonadLiftT m n] [Monad n]
+    [Finite α m] :
+    ForIn n (IterM.Total (α := α) m β) β :=
+  haveI : ForIn' n (IterM.Total (α := α) m β) β _ := IterM.Total.instForIn'
+  instForInOfForIn'
+
+instance {m : Type w → Type w'} {n : Type w → Type w''} {α : Type w} {β : Type w} [Iterator α m β]
+    [IteratorLoop α m n] [Monad n] [MonadLiftT m n] : ForM n (IterM (α := α) m β) β where
   forM it f := forIn it PUnit.unit (fun out _ => do f out; return .yield .unit)
 
-instance {m : Type w → Type w'} {n : Type w → Type w''}
-    {α : Type w} {β : Type w} [Iterator α m β] [IteratorLoopPartial α m n] [Monad n]
-    [MonadLiftT m n] :
+instance {m : Type w → Type w'} {n : Type w → Type w''} {α : Type w} {β : Type w} [Monad n]
+    [Iterator α m β] [IteratorLoop α m n] [MonadLiftT m n] :
     ForM n (IterM.Partial (α := α) m β) β where
+  forM it f := forIn it PUnit.unit (fun out _ => do f out; return .yield .unit)
+
+instance {m : Type w → Type w'} {n : Type w → Type w''} {α : Type w} {β : Type w} [Iterator α m β]
+    [IteratorLoop α m n] [Monad n] [MonadLiftT m n] [Finite α m] :
+    ForM n (IterM.Total (α := α) m β) β where
   forM it f := forIn it PUnit.unit (fun out _ => do f out; return .yield .unit)
 
 /--
@@ -305,15 +266,10 @@ The accumulated value is combined with the each element of the list in order, us
 
 The monadic effects of `f` are interleaved with potential effects caused by the iterator's step
 function. Therefore, it may *not* be equivalent to `(← it.toList).foldlM`.
-
-This function requires a `Finite` instance proving that the iterator will finish after a finite
-number of steps. If the iterator is not finite or such an instance is not available, consider using
-`it.allowNontermination.foldM` instead of `it.foldM`. However, it is not possible to formally
-verify the behavior of the partial variant.
 -/
 @[always_inline, inline]
 def IterM.foldM {m : Type w → Type w'} {n : Type w → Type w''} [Monad n]
-    {α : Type w} {β : Type w} {γ : Type w} [Iterator α m β] [Finite α m] [IteratorLoop α m n]
+    {α : Type w} {β : Type w} {γ : Type w} [Iterator α m β] [IteratorLoop α m n]
     [MonadLiftT m n]
     (f : γ → β → n γ) (init : γ) (it : IterM (α := α) m β) : n γ :=
   ForIn.forIn it init (fun x acc => ForInStep.yield <$> f acc x)
@@ -325,31 +281,40 @@ The accumulated value is combined with the each element of the list in order, us
 The monadic effects of `f` are interleaved with potential effects caused by the iterator's step
 function. Therefore, it may *not* be equivalent to `it.toList.foldlM`.
 
-This is a partial, potentially nonterminating, function. It is not possible to formally verify
-its behavior. If the iterator has a `Finite` instance, consider using `IterM.foldM` instead.
+This function is deprecated. Instead of `it.allowNontermination.foldM`, use `it.foldM`.
 -/
-@[always_inline, inline]
+@[always_inline, inline, deprecated IterM.foldM (since := "2025-12-04")]
 def IterM.Partial.foldM {m : Type w → Type w'} {n : Type w → Type w'} [Monad n]
-    {α : Type w} {β : Type w} {γ : Type w} [Iterator α m β] [IteratorLoopPartial α m n]
-    [MonadLiftT m n]
+    {α : Type w} {β : Type w} {γ : Type w} [Iterator α m β] [IteratorLoop α m n] [MonadLiftT m n]
     (f : γ → β → n γ) (init : γ) (it : IterM.Partial (α := α) m β) : n γ :=
   ForIn.forIn it init (fun x acc => ForInStep.yield <$> f acc x)
 
 /--
+Folds a monadic function over an iterator from the left, accumulating a value starting with `init`.
+The accumulated value is combined with the each element of the list in order, using `f`.
+
+The monadic effects of `f` are interleaved with potential effects caused by the iterator's step
+function. Therefore, it may *not* be equivalent to `it.toList.foldlM`.
+
+This variant terminates after finitely many steps and requires a proof that the iterator is
+finite. If such a proof is not available, consider using `IterM.foldM`.
+-/
+@[always_inline, inline]
+def IterM.Total.foldM {m : Type w → Type w'} {n : Type w → Type w'} [Monad n]
+    {α : Type w} {β : Type w} {γ : Type w} [Iterator α m β] [IteratorLoop α m n] [MonadLiftT m n]
+    [Finite α m] (f : γ → β → n γ) (init : γ) (it : IterM.Total (α := α) m β) : n γ :=
+  it.it.foldM (init := init) f
+
+/--
 Folds a function over an iterator from the left, accumulating a value starting with `init`.
 The accumulated value is combined with the each element of the list in order, using `f`.
 
 It is equivalent to `it.toList.foldl`.
-
-This function requires a `Finite` instance proving that the iterator will finish after a finite
-number of steps. If the iterator is not finite or such an instance is not available, consider using
-`it.allowNontermination.fold` instead of `it.fold`. However, it is not possible to formally
-verify the behavior of the partial variant.
 -/
 @[always_inline, inline]
 def IterM.fold {m : Type w → Type w'} {α : Type w} {β : Type w} {γ : Type w} [Monad m]
-    [Iterator α m β] [Finite α m] [IteratorLoop α m m]
-    (f : γ → β → γ) (init : γ) (it : IterM (α := α) m β) : m γ :=
+    [Iterator α m β] [IteratorLoop α m m] (f : γ → β → γ) (init : γ) (it : IterM (α := α) m β) :
+    m γ :=
   ForIn.forIn (m := m) it init (fun x acc => pure (ForInStep.yield (f acc x)))
 
 /--
@@ -358,27 +323,36 @@ The accumulated value is combined with the each element of the list in order, us
 
 It is equivalent to `it.toList.foldl`.
 
-This is a partial, potentially nonterminating, function. It is not possible to formally verify
-its behavior. If the iterator has a `Finite` instance, consider using `IterM.fold` instead.
+This function is deprecated. Instead of `it.allowNontermination.fold`, use `it.fold`.
 -/
-@[always_inline, inline]
+@[always_inline, inline, deprecated IterM.Partial.fold (since := "2025-12-04")]
 def IterM.Partial.fold {m : Type w → Type w'} {α : Type w} {β : Type w} {γ : Type w}
-    [Monad m] [Iterator α m β] [IteratorLoopPartial α m m]
-    (f : γ → β → γ) (init : γ) (it : IterM.Partial (α := α) m β) : m γ :=
+    [Monad m] [Iterator α m β] [IteratorLoop α m m] (f : γ → β → γ) (init : γ)
+    (it : IterM.Partial (α := α) m β) : m γ :=
   ForIn.forIn (m := m) it init (fun x acc => pure (ForInStep.yield (f acc x)))
 
 /--
+Folds a function over an iterator from the left, accumulating a value starting with `init`.
+The accumulated value is combined with the each element of the list in order, using `f`.
+
+It is equivalent to `it.toList.foldl`.
+
+This variant terminates after finitely many steps and requires a proof that the iterator is
+finite. If such a proof is not available, consider using `IterM.fold`.
+-/
+@[always_inline, inline]
+def IterM.Total.fold {m : Type w → Type w'} {α : Type w} {β : Type w} {γ : Type w}
+    [Monad m] [Iterator α m β] [IteratorLoop α m m] [Finite α m] (f : γ → β → γ) (init : γ)
+    (it : IterM.Total (α := α) m β) : m γ :=
+  it.it.fold (init := init) f
+
+/--
 Iterates over the whole iterator, applying the monadic effects of each step, discarding all
 emitted values.
-
-This function requires a `Finite` instance proving that the iterator will finish after a finite
-number of steps. If the iterator is not finite or such an instance is not available, consider using
-`it.allowNontermination.drain` instead of `it.drain`. However, it is not possible to formally
-verify the behavior of the partial variant.
 -/
 @[always_inline, inline]
 def IterM.drain {α : Type w} {m : Type w → Type w'} [Monad m] {β : Type w}
-    [Iterator α m β] [Finite α m] (it : IterM (α := α) m β) [IteratorLoop α m m] :
+    [Iterator α m β] (it : IterM (α := α) m β) [IteratorLoop α m m] :
     m PUnit :=
   it.fold (γ := PUnit) (fun _ _ => .unit) .unit
 
@@ -386,31 +360,36 @@ def IterM.drain {α : Type w} {m : Type w → Type w'} [Monad m] {β : Type w}
 Iterates over the whole iterator, applying the monadic effects of each step, discarding all
 emitted values.
 
-This is a partial, potentially nonterminating, function. It is not possible to formally verify
-its behavior. If the iterator has a `Finite` instance, consider using `IterM.drain` instead.
+This function is deprecated. Instead of `it.allowNontermination.drain`, use `it.drain`.
+-/
+@[always_inline, inline, deprecated IterM.drain (since := "2025-12-04")]
+def IterM.Partial.drain {α : Type w} {m : Type w → Type w'} [Monad m] {β : Type w}
+    [Iterator α m β] (it : IterM.Partial (α := α) m β) [IteratorLoop α m m] : m PUnit :=
+  it.it.fold (γ := PUnit) (fun _ _ => .unit) .unit
+
+/--
+Iterates over the whole iterator, applying the monadic effects of each step, discarding all
+emitted values.
+
+This variant terminates after finitely many steps and requires a proof that the iterator is
+finite. If such a proof is not available, consider using `IterM.drain`.
 -/
 @[always_inline, inline]
-def IterM.Partial.drain {α : Type w} {m : Type w → Type w'} [Monad m] {β : Type w}
-    [Iterator α m β] (it : IterM.Partial (α := α) m β) [IteratorLoopPartial α m m] :
-    m PUnit :=
-  it.fold (γ := PUnit) (fun _ _ => .unit) .unit
+def IterM.Total.drain {α : Type w} {m : Type w → Type w'} [Monad m] {β : Type w}
+    [Iterator α m β] [Finite α m] (it : IterM.Total (α := α) m β) [IteratorLoop α m m] : m PUnit :=
+  it.it.drain
 
 set_option doc.verso true in
 /--
 Returns {lean}`ULift.up true` if the monadic predicate {name}`p` returns {lean}`ULift.up true` for
 any element emitted by the iterator {name}`it`.
 
-{lit}`O(|xs|)`. Short-circuits upon encountering the first match. The elements in {name}`it` are
+{lit}`O(|it|)`. Short-circuits upon encountering the first match. The outputs of {name}`it` are
 examined in order of iteration.
-
-This function requires a {name}`Finite` instance proving that the iterator will finish after a
-finite number of steps. If the iterator is not finite or such an instance is not available,
-consider using {lit}`it.allowNontermination.anyM` instead of {lean}`it.anyM`. However, it is not
-possible to formally verify the behavior of the partial variant.
 -/
 @[specialize]
 def IterM.anyM {α β : Type w} {m : Type w → Type w'} [Monad m]
-    [Iterator α m β] [IteratorLoop α m m] [Finite α m]
+    [Iterator α m β] [IteratorLoop α m m]
     (p : β → m (ULift Bool)) (it : IterM (α := α) m β) : m (ULift Bool) :=
   ForIn.forIn it (ULift.up false) (fun x _ => do
     if (← p x).down then
@@ -423,39 +402,45 @@ set_option doc.verso true in
 Returns {lean}`ULift.up true` if the monadic predicate {name}`p` returns {lean}`ULift.up true` for
 any element emitted by the iterator {name}`it`.
 
-{lit}`O(|xs|)`. Short-circuits upon encountering the first match. The elements in {name}`it` are
+{lit}`O(|it|)`. Short-circuits upon encountering the first match. The outputs of {name}`it` are
 examined in order of iteration.
 
-This is a partial, potentially nonterminating, function. It is not possible to formally verify
-its behavior. If the iterator has a {name}`Finite` instance, consider using {name}`IterM.anyM`
-instead.
+This function is deprecated. Instead of {lit}`it.allowNontermination.anyM`, use {lit}`it.anyM`.
 -/
-@[specialize]
+@[always_inline, inline, deprecated IterM.anyM (since := "2025-12-04")]
 def IterM.Partial.anyM {α β : Type w} {m : Type w → Type w'} [Monad m]
-    [Iterator α m β] [IteratorLoopPartial α m m]
-    (p : β → m (ULift Bool)) (it : IterM.Partial (α := α) m β) : m (ULift Bool) :=
-  ForIn.forIn it (ULift.up false) (fun x _ => do
-    if (← p x).down then
-      return .done (.up true)
-    else
-      return .yield (.up false))
+    [Iterator α m β] [IteratorLoop α m m] (p : β → m (ULift Bool))
+    (it : IterM.Partial (α := α) m β) : m (ULift Bool) :=
+  it.it.anyM p
+
+set_option doc.verso true in
+/--
+Returns {lean}`ULift.up true` if the monadic predicate {name}`p` returns {lean}`ULift.up true` for
+any element emitted by the iterator {name}`it`.
+
+{lit}`O(|it|)`. Short-circuits upon encountering the first match. The outputs of {name}`it` are
+examined in order of iteration.
+
+This variant terminates after finitely many steps and requires a proof that the iterator is
+finite. If such a proof is not available, consider using {name}`IterM.anyM`.
+-/
+@[always_inline, inline]
+def IterM.Total.anyM {α β : Type w} {m : Type w → Type w'} [Monad m]
+    [Iterator α m β] [IteratorLoop α m m] [Finite α m] (p : β → m (ULift Bool))
+    (it : IterM.Total (α := α) m β) : m (ULift Bool) :=
+  it.it.anyM p
 
 set_option doc.verso true in
 /--
 Returns {lean}`ULift.up true` if the pure predicate {name}`p` returns {lean}`true` for
 any element emitted by the iterator {name}`it`.
 
-{lit}`O(|xs|)`. Short-circuits upon encountering the first match. The elements in {name}`it` are
+{lit}`O(|it|)`. Short-circuits upon encountering the first match. The outputs of {name}`it` are
 examined in order of iteration.
-
-This function requires a {name}`Finite` instance proving that the iterator will finish after a
-finite number of steps. If the iterator is not finite or such an instance is not available,
-consider using {lit}`it.allowNontermination.any` instead of {lean}`it.any`. However, it is not
-possible to formally verify the behavior of the partial variant.
 -/
 @[inline]
 def IterM.any {α β : Type w} {m : Type w → Type w'} [Monad m]
-    [Iterator α m β] [IteratorLoop α m m] [Finite α m]
+    [Iterator α m β] [IteratorLoop α m m]
     (p : β → Bool) (it : IterM (α := α) m β) : m (ULift Bool) := do
   it.anyM (fun x => pure (.up (p x)))
 
@@ -464,79 +449,96 @@ set_option doc.verso true in
 Returns {lean}`ULift.up true` if the pure predicate {name}`p` returns {lean}`true` for
 any element emitted by the iterator {name}`it`.
 
-{lit}`O(|xs|)`. Short-circuits upon encountering the first match. The elements in {name}`it` are
+{lit}`O(|it|)`. Short-circuits upon encountering the first match. The outputs of {name}`it` are
 examined in order of iteration.
 
-This is a partial, potentially nonterminating, function. It is not possible to formally verify
-its behavior. If the iterator has a {name}`Finite` instance, consider using {name}`IterM.any`
-instead.
+This function is deprecated. Instead of {lit}`it.allowNontermination.any`, use {lit}`it.any`.
+-/
+@[inline, deprecated IterM.any (since := "2025-12-04")]
+def IterM.Partial.any {α β : Type w} {m : Type w → Type w'} [Monad m] [Iterator α m β]
+    [IteratorLoop α m m] (p : β → Bool) (it : IterM.Partial (α := α) m β) : m (ULift Bool) := do
+  it.it.any p
+
+set_option doc.verso true in
+/--
+Returns {lean}`ULift.up true` if the pure predicate {name}`p` returns {lean}`true` for
+any element emitted by the iterator {name}`it`.
+
+{lit}`O(|it|)`. Short-circuits upon encountering the first match. The outputs of {name}`it` are
+examined in order of iteration.
+
+This variant terminates after finitely many steps and requires a proof that the iterator is
+finite. If such a proof is not available, consider using {name}`IterM.any`.
 -/
 @[inline]
-def IterM.Partial.any {α β : Type w} {m : Type w → Type w'} [Monad m]
-    [Iterator α m β] [IteratorLoopPartial α m m]
-    (p : β → Bool) (it : IterM.Partial (α := α) m β) : m (ULift Bool) := do
-  it.anyM (fun x => pure (.up (p x)))
+def IterM.Total.any {α β : Type w} {m : Type w → Type w'} [Monad m] [Iterator α m β]
+    [IteratorLoop α m m] [Finite α m] (p : β → Bool) (it : IterM.Total (α := α) m β) :
+    m (ULift Bool) := do
+  it.it.any p
 
 set_option doc.verso true in
 /--
 Returns {lean}`ULift.up true` if the monadic predicate {name}`p` returns {lean}`ULift.up true` for
 all elements emitted by the iterator {name}`it`.
 
-{lit}`O(|xs|)`. Short-circuits upon encountering the first mismatch. The elements in {name}`it` are
+{lit}`O(|it|)`. Short-circuits upon encountering the first mismatch. The outputs of {name}`it` are
 examined in order of iteration.
-
-This function requires a {name}`Finite` instance proving that the iterator will finish after a
-finite number of steps. If the iterator is not finite or such an instance is not available,
-consider using {lit}`it.allowNontermination.allM` instead of {lean}`it.allM`. However, it is not
-possible to formally verify the behavior of the partial variant.
 -/
 @[specialize]
-def IterM.allM {α β : Type w} {m : Type w → Type w'} [Monad m]
-    [Iterator α m β] [IteratorLoop α m m] [Finite α m]
+def IterM.allM {α β : Type w} {m : Type w → Type w'} [Monad m] [Iterator α m β] [IteratorLoop α m m]
     (p : β → m (ULift Bool)) (it : IterM (α := α) m β) : m (ULift Bool) := do
   ForIn.forIn it (ULift.up true) (fun x _ => do
     if (← p x).down then
       return .yield (.up true)
     else
       return .done (.up false))
+
 set_option doc.verso true in
 /--
 Returns {lean}`ULift.up true` if the monadic predicate {name}`p` returns {lean}`ULift.up true` for
 all elements emitted by the iterator {name}`it`.
 
-{lit}`O(|xs|)`. Short-circuits upon encountering the first mismatch. The elements in {name}`it` are
+{lit}`O(|it|)`. Short-circuits upon encountering the first mismatch. The outputs of {name}`it` are
 examined in order of iteration.
 
-This is a partial, potentially nonterminating, function. It is not possible to formally verify
-its behavior. If the iterator has a {name}`Finite` instance, consider using {name}`IterM.allM`
-instead.
+This function is deprecated. Instead of {lit}`it.allowNontermination.allM`, use {lit}`it.allM`.
 -/
-@[specialize]
-def IterM.Partial.allM {α β : Type w} {m : Type w → Type w'} [Monad m]
-    [Iterator α m β] [IteratorLoopPartial α m m]
-    (p : β → m (ULift Bool)) (it : IterM.Partial (α := α) m β) : m (ULift Bool) := do
-  ForIn.forIn it (ULift.up true) (fun x _ => do
-    if (← p x).down then
-      return .yield (.up true)
-    else
-      return .done (.up false))
+@[always_inline, inline, deprecated IterM.allM (since := "2025-12-04")]
+def IterM.Partial.allM {α β : Type w} {m : Type w → Type w'} [Monad m] [Iterator α m β]
+    [IteratorLoop α m m] (p : β → m (ULift Bool)) (it : IterM.Partial (α := α) m β) :
+    m (ULift Bool) := do
+  it.it.allM p
+
+set_option doc.verso true in
+/--
+Returns {lean}`ULift.up true` if the monadic predicate {name}`p` returns {lean}`ULift.up true` for
+all elements emitted by the iterator {name}`it`.
+
+{lit}`O(|it|)`. Short-circuits upon encountering the first mismatch. The outputs of {name}`it` are
+examined in order of iteration.
+
+This variant terminates after finitely many steps and requires a proof that the iterator is
+finite. If such a proof is not available, consider using {name}`IterM.allM`.
+-/
+@[always_inline, inline]
+def IterM.Total.allM {α β : Type w} {m : Type w → Type w'} [Monad m] [Iterator α m β]
+    [IteratorLoop α m m] [Finite α m] (p : β → m (ULift Bool)) (it : IterM.Total (α := α) m β) :
+    m (ULift Bool) := do
+  it.it.allM p
 
 set_option doc.verso true in
 /--
 Returns {lean}`ULift.up true` if the pure predicate {name}`p` returns {lean}`true` for
 all elements emitted by the iterator {name}`it`.
 
-{lit}`O(|xs|)`. Short-circuits upon encountering the first mismatch. The elements in {name}`it` are
+{lit}`O(|it|)`. Short-circuits upon encountering the first mismatch. The outputs of {name}`it` are
 examined in order of iteration.
 
-This function requires a {name}`Finite` instance proving that the iterator will finish after a
-finite number of steps. If the iterator is not finite or such an instance is not available,
-consider using {lit}`it.allowNontermination.all` instead of {lean}`it.all`. However, it is not
-possible to formally verify the behavior of the partial variant.
+If the iterator is not finite, this function might run forever. The variant
+{lit}`it.ensureTermination.toListRev` always terminates after finitely many steps.
 -/
 @[inline]
-def IterM.all {α β : Type w} {m : Type w → Type w'} [Monad m]
-    [Iterator α m β] [IteratorLoop α m m] [Finite α m]
+def IterM.all {α β : Type w} {m : Type w → Type w'} [Monad m] [Iterator α m β] [IteratorLoop α m m]
     (p : β → Bool) (it : IterM (α := α) m β) : m (ULift Bool) := do
   it.allM (fun x => pure (.up (p x)))
 
@@ -545,72 +547,349 @@ set_option doc.verso true in
 Returns {lean}`ULift.up true` if the pure predicate {name}`p` returns {lean}`true` for
 all elements emitted by the iterator {name}`it`.
 
-{lit}`O(|xs|)`. Short-circuits upon encountering the first mismatch. The elements in {name}`it` are
+{lit}`O(|it|)`. Short-circuits upon encountering the first mismatch. The outputs of {name}`it` are
 examined in order of iteration.
 
-This is a partial, potentially nonterminating, function. It is not possible to formally verify
-its behavior. If the iterator has a {name}`Finite` instance, consider using {name}`IterM.all`
-instead.
+This function is deprecated. Instead of {lit}`it.allowNontermination.allM`, use {lit}`it.allM`.
+-/
+@[inline, deprecated IterM.all (since := "2025-12-04")]
+def IterM.Partial.all {α β : Type w} {m : Type w → Type w'} [Monad m] [Iterator α m β]
+    [IteratorLoop α m m] (p : β → Bool) (it : IterM.Partial (α := α) m β) : m (ULift Bool) := do
+  it.it.all p
+
+set_option doc.verso true in
+/--
+Returns {lean}`ULift.up true` if the pure predicate {name}`p` returns {lean}`true` for
+all elements emitted by the iterator {name}`it`.
+
+{lit}`O(|it|)`. Short-circuits upon encountering the first mismatch. The outputs of {name}`it` are
+examined in order of iteration.
+
+This variant terminates after finitely many steps and requires a proof that the iterator is
+finite. If such a proof is not available, consider using {name}`IterM.all`.
 -/
 @[inline]
-def IterM.Partial.all {α β : Type w} {m : Type w → Type w'} [Monad m]
-    [Iterator α m β] [IteratorLoopPartial α m m]
-    (p : β → Bool) (it : IterM.Partial (α := α) m β) : m (ULift Bool) := do
-  it.allM (fun x => pure (.up (p x)))
+def IterM.Total.all {α β : Type w} {m : Type w → Type w'} [Monad m] [Iterator α m β]
+    [IteratorLoop α m m] [Finite α m] (p : β → Bool) (it : IterM.Total (α := α) m β) :
+    m (ULift Bool) := do
+  it.it.all p
 
+/--
+Returns the first non-`none` result of applying the monadic function `f` to each output
+of the iterator, in order. Returns `none` if `f` returns `none` for all outputs.
+
+`O(|it|)`. Short-circuits when `f` returns `some _`. The outputs of `it` are
+examined in order of iteration.
+
+If the iterator is not finite, this function might run forever. The variant
+`it.ensureTermination.findSomeM?` always terminates after finitely many steps.
+
+Example:
+```lean example
+#eval ([7, 6, 5, 8, 1, 2, 6].iterM IO).findSomeM? fun i => do
+  if i < 5 then
+    return some (i * 10)
+  if i ≤ 6 then
+    IO.println s!"Almost! {i}"
+  return none
+```
+```output
+Almost! 6
+Almost! 5
+```
+```output
+some 10
+```
+-/
 @[inline]
 def IterM.findSomeM? {α β γ : Type w} {m : Type w → Type w'} [Monad m] [Iterator α m β]
-    [IteratorLoop α m m] [Finite α m] (it : IterM (α := α) m β) (f : β → m (Option γ)) :
+    [IteratorLoop α m m] (it : IterM (α := α) m β) (f : β → m (Option γ)) :
     m (Option γ) :=
   ForIn.forIn it none (fun x _ => do
     match ← f x with
     | none => return .yield none
     | some fx => return .done (some fx))
 
-@[inline]
+/--
+Returns the first non-`none` result of applying the monadic function `f` to each output
+of the iterator, in order. Returns `none` if `f` returns `none` for all outputs.
+
+`O(|it|)`. Short-circuits when `f` returns `some _`. The outputs of `it` are
+examined in order of iteration.
+
+This function is deprecated. Instead of `it.allowNontermination.findSomeM?`, use `it.findSomeM?`.
+
+Example:
+```lean example
+#eval ([7, 6, 5, 8, 1, 2, 6].iterM IO).findSomeM? fun i => do
+  if i < 5 then
+    return some (i * 10)
+  if i ≤ 6 then
+    IO.println s!"Almost! {i}"
+  return none
+```
+```output
+Almost! 6
+Almost! 5
+```
+```output
+some 10
+```
+-/
+@[inline, deprecated IterM.findSomeM? (since := "2025-12-04")]
 def IterM.Partial.findSomeM? {α β γ : Type w} {m : Type w → Type w'} [Monad m] [Iterator α m β]
-    [IteratorLoopPartial α m m] (it : IterM.Partial (α := α) m β) (f : β → m (Option γ)) :
+    [IteratorLoop α m m] (it : IterM.Partial (α := α) m β) (f : β → m (Option γ)) :
     m (Option γ) :=
-  ForIn.forIn it none (fun x _ => do
-    match ← f x with
-    | none => return .yield none
-    | some fx => return .done (some fx))
+  it.it.findSomeM? f
 
+/--
+Returns the first non-`none` result of applying the monadic function `f` to each output
+of the iterator, in order. Returns `none` if `f` returns `none` for all outputs.
+
+`O(|it|)`. Short-circuits when `f` returns `some _`. The outputs of `it` are
+examined in order of iteration.
+
+This variant terminates after finitely many steps and requires a proof that the iterator is
+finite. If such a proof is not available, consider using `IterM.findSomeM?`.
+
+Example:
+```lean example
+#eval ([7, 6, 5, 8, 1, 2, 6].iterM IO).findSomeM? fun i => do
+  if i < 5 then
+    return some (i * 10)
+  if i ≤ 6 then
+    IO.println s!"Almost! {i}"
+  return none
+```
+```output
+Almost! 6
+Almost! 5
+```
+```output
+some 10
+```
+-/
+@[inline]
+def IterM.Total.findSomeM? {α β γ : Type w} {m : Type w → Type w'} [Monad m] [Iterator α m β]
+    [IteratorLoop α m m] [Finite α m] (it : IterM.Total (α := α) m β) (f : β → m (Option γ)) :
+    m (Option γ) :=
+  it.it.findSomeM? f
+
+/--
+Returns the first non-`none` result of applying `f` to each output of the iterator, in order.
+Returns `none` if `f` returns `none` for all outputs.
+
+`O(|it|)`. Short-circuits when `f` returns `some _`.The outputs of `it` are examined in order of
+iteration.
+
+If the iterator is not finite, this function might run forever. The variant
+`it.ensureTermination.findSome?` always terminates after finitely many steps.
+
+Examples:
+ * `([7, 6, 5, 8, 1, 2, 6].iterM Id).findSome? (fun x => if x < 5 then some (10 * x) else none) = pure (some 10)`
+ * `([7, 6, 5, 8, 1, 2, 6].iterM Id).findSome? (fun x => if x < 1 then some (10 * x) else none) = pure none`
+-/
 @[inline]
 def IterM.findSome? {α β γ : Type w} {m : Type w → Type w'} [Monad m] [Iterator α m β]
-    [IteratorLoop α m m] [Finite α m] (it : IterM (α := α) m β) (f : β → Option γ) :
+    [IteratorLoop α m m] (it : IterM (α := α) m β) (f : β → Option γ) :
     m (Option γ) :=
   it.findSomeM? (pure <| f ·)
 
-@[inline]
+/--
+Returns the first non-`none` result of applying `f` to each output of the iterator, in order.
+Returns `none` if `f` returns `none` for all outputs.
+
+`O(|it|)`. Short-circuits when `f` returns `some _`.The outputs of `it` are examined in order of
+iteration.
+
+This function is deprecated. Instead of `it.allowNontermination.findSome?`, use `it.findSome?`.
+
+Examples:
+ * `([7, 6, 5, 8, 1, 2, 6].iterM Id).allowNontermination.findSome? (fun x => if x < 5 then some (10 * x) else none) = pure (some 10)`
+ * `([7, 6, 5, 8, 1, 2, 6].iterM Id).allowNontermination.findSome? (fun x => if x < 1 then some (10 * x) else none) = pure none`
+-/
+@[inline, deprecated IterM.findSome? (since := "2025-12-04")]
 def IterM.Partial.findSome? {α β γ : Type w} {m : Type w → Type w'} [Monad m] [Iterator α m β]
-    [IteratorLoopPartial α m m] (it : IterM.Partial (α := α) m β) (f : β → Option γ) :
+    [IteratorLoop α m m] (it : IterM.Partial (α := α) m β) (f : β → Option γ) :
     m (Option γ) :=
-  it.findSomeM? (pure <| f ·)
+  it.it.findSome? f
 
+/--
+Returns the first non-`none` result of applying `f` to each output of the iterator, in order.
+Returns `none` if `f` returns `none` for all outputs.
+
+`O(|it|)`. Short-circuits when `f` returns `some _`.The outputs of `it` are examined in order of
+iteration.
+
+This variant terminates after finitely many steps and requires a proof that the iterator is
+finite. If such a proof is not available, consider using `IterM.findSome?`.
+
+Examples:
+ * `([7, 6, 5, 8, 1, 2, 6].iterM Id).ensureTermination.findSome? (fun x => if x < 5 then some (10 * x) else none) = pure (some 10)`
+ * `([7, 6, 5, 8, 1, 2, 6].iterM Id).ensureTermination.findSome? (fun x => if x < 1 then some (10 * x) else none) = pure none`
+-/
+@[inline]
+def IterM.Total.findSome? {α β γ : Type w} {m : Type w → Type w'} [Monad m] [Iterator α m β]
+    [IteratorLoop α m m] [Finite α m] (it : IterM.Partial (α := α) m β) (f : β → Option γ) :
+    m (Option γ) :=
+  it.it.findSome? f
+
+/--
+Returns the first output of the iterator for which the monadic predicate `p` returns `true`, or
+`none` if no such element is found.
+
+`O(|it|)`. Short-circuits when `f` returns `true`. The outputs of `it` are examined in order of
+iteration.
+
+If the iterator is not finite, this function might run forever. The variant
+`it.ensureTermination.findM?` always terminates after finitely many steps.
+
+Example:
+```lean example
+#eval ([7, 6, 5, 8, 1, 2, 6].iterM IO).findM? fun i => do
+  if i < 5 then
+    return true
+  if i ≤ 6 then
+    IO.println s!"Almost! {i}"
+  return false
+```
+```output
+Almost! 6
+Almost! 5
+```
+```output
+some 1
+```
+-/
 @[inline]
 def IterM.findM? {α β : Type w} {m : Type w → Type w'} [Monad m] [Iterator α m β]
-    [IteratorLoop α m m] [Finite α m] (it : IterM (α := α) m β) (f : β → m (ULift Bool)) :
+    [IteratorLoop α m m] (it : IterM (α := α) m β) (f : β → m (ULift Bool)) :
     m (Option β) :=
   it.findSomeM? (fun x => return if (← f x).down then some x else none)
 
-@[inline]
+/--
+Returns the first output of the iterator for which the monadic predicate `p` returns `true`, or
+`none` if no such element is found.
+
+`O(|it|)`. Short-circuits when `f` returns `true`. The outputs of `it` are examined in order of
+iteration.
+
+This function is deprecated. Instead of `it.allowNontermination.findM?`, use `it.findM?`.
+
+Example:
+```lean example
+#eval ([7, 6, 5, 8, 1, 2, 6].iterM IO).findM? fun i => do
+  if i < 5 then
+    return true
+  if i ≤ 6 then
+    IO.println s!"Almost! {i}"
+  return false
+```
+```output
+Almost! 6
+Almost! 5
+```
+```output
+some 1
+```
+-/
+@[inline, deprecated IterM.findM? (since := "2025-12-04")]
 def IterM.Partial.findM? {α β : Type w} {m : Type w → Type w'} [Monad m] [Iterator α m β]
-    [IteratorLoopPartial α m m] (it : IterM.Partial (α := α) m β) (f : β → m (ULift Bool)) :
+    [IteratorLoop α m m] (it : IterM.Partial (α := α) m β) (f : β → m (ULift Bool)) :
     m (Option β) :=
-  it.findSomeM? (fun x => return if (← f x).down then some x else none)
+  it.it.findM? f
 
+/--
+Returns the first output of the iterator for which the monadic predicate `p` returns `true`, or
+`none` if no such element is found.
+
+`O(|it|)`. Short-circuits when `f` returns `true`. The outputs of `it` are examined in order of
+iteration.
+
+This variant requires terminates after finitely many steps and requires a proof that the iterator is
+finite. If such a proof is not available, consider using `IterM.findM?`.
+
+Example:
+```lean example
+#eval ([7, 6, 5, 8, 1, 2, 6].iterM IO).findM? fun i => do
+  if i < 5 then
+    return true
+  if i ≤ 6 then
+    IO.println s!"Almost! {i}"
+  return false
+```
+```output
+Almost! 6
+Almost! 5
+```
+```output
+some 1
+```
+-/
+@[inline]
+def IterM.Total.findM? {α β : Type w} {m : Type w → Type w'} [Monad m] [Iterator α m β]
+    [IteratorLoop α m m] [Finite α m] (it : IterM.Total (α := α) m β) (f : β → m (ULift Bool)) :
+    m (Option β) :=
+  it.it.findM? f
+
+/--
+Returns the first output of the iterator for which the predicate `p` returns `true`, or `none` if
+no such output is found.
+
+`O(|it|)`. Short-circuits upon encountering the first match. The elements in `it` are examined in
+order of iteration.
+
+If the iterator is not finite, this function might run forever. The variant
+`it.ensureTermination.find?` always terminates after finitely many steps.
+
+Examples:
+* `([7, 6, 5, 8, 1, 2, 6].iterM Id).find? (· < 5) = pure (some 1)`
+* `([7, 6, 5, 8, 1, 2, 6].iterM Id).find? (· < 1) = pure none`
+-/
 @[inline]
 def IterM.find? {α β : Type w} {m : Type w → Type w'} [Monad m] [Iterator α m β]
-    [IteratorLoop α m m] [Finite α m] (it : IterM (α := α) m β) (f : β → Bool) :
+    [IteratorLoop α m m] (it : IterM (α := α) m β) (f : β → Bool) :
     m (Option β) :=
   it.findM? (pure <| .up <| f ·)
 
-@[inline]
+/--
+Returns the first output of the iterator for which the predicate `p` returns `true`, or `none` if
+no such output is found.
+
+`O(|it|)`. Short-circuits upon encountering the first match. The elements in `it` are examined in
+order of iteration.
+
+This function is deprecated. Instead of `it.allowNontermination.find?`, use `it.find?`.
+
+Examples:
+* `([7, 6, 5, 8, 1, 2, 6].iterM Id).allowNontermination.find? (· < 5) = pure (some 1)`
+* `([7, 6, 5, 8, 1, 2, 6].iterM Id).allowNontermination.find? (· < 1) = pure none`
+-/
+@[inline, deprecated IterM.find? (since := "2025-12-04")]
 def IterM.Partial.find? {α β : Type w} {m : Type w → Type w'} [Monad m] [Iterator α m β]
-    [IteratorLoopPartial α m m] (it : IterM.Partial (α := α) m β) (f : β → Bool) :
+    [IteratorLoop α m m] (it : IterM.Partial (α := α) m β) (f : β → Bool) :
     m (Option β) :=
-  it.findM? (pure <| .up <| f ·)
+  it.it.find? f
+
+/--
+Returns the first output of the iterator for which the predicate `p` returns `true`, or `none` if
+no such output is found.
+
+`O(|it|)`. Short-circuits upon encountering the first match. The elements in `it` are examined in
+order of iteration.
+
+This variant terminates after finitely many steps and requires a proof that the iterator is
+finite. If such a proof is not available, consider using `IterM.find?`.
+
+Examples:
+* `([7, 6, 5, 8, 1, 2, 6].iterM Id).find? (· < 5) = pure (some 1)`
+* `([7, 6, 5, 8, 1, 2, 6].iterM Id).find? (· < 1) = pure none`
+-/
+@[inline]
+def IterM.Total.find? {α β : Type w} {m : Type w → Type w'} [Monad m] [Iterator α m β]
+    [IteratorLoop α m m] [Finite α m] (it : IterM.Total (α := α) m β) (f : β → Bool) :
+    m (Option β) :=
+  it.it.find? f
 
 section Count
 
@@ -622,9 +901,8 @@ Steps through the whole iterator, counting the number of outputs emitted.
 This function's runtime is linear in the number of steps taken by the iterator.
 -/
 @[always_inline, inline]
-def IterM.count {α : Type w} {m : Type w → Type w'} {β : Type w} [Iterator α m β] [Finite α m]
-    [IteratorLoop α m m]
-    [Monad m] (it : IterM (α := α) m β) : m (ULift Nat) :=
+def IterM.count {α : Type w} {m : Type w → Type w'} {β : Type w} [Iterator α m β]
+    [IteratorLoop α m m] [Monad m] (it : IterM (α := α) m β) : m (ULift Nat) :=
   it.fold (init := .up 0) fun acc _ => .up (acc.down + 1)
 
 /--
@@ -635,9 +913,8 @@ Steps through the whole iterator, counting the number of outputs emitted.
 This function's runtime is linear in the number of steps taken by the iterator.
 -/
 @[always_inline, inline, deprecated IterM.count (since := "2025-10-29")]
-def IterM.size {α : Type w} {m : Type w → Type w'} {β : Type w} [Iterator α m β] [Finite α m]
-    [IteratorLoop α m m]
-    [Monad m] (it : IterM (α := α) m β) : m (ULift Nat) :=
+def IterM.size {α : Type w} {m : Type w → Type w'} {β : Type w} [Iterator α m β]
+    [IteratorLoop α m m] [Monad m] (it : IterM (α := α) m β) : m (ULift Nat) :=
   it.count
 
 /--
@@ -647,10 +924,10 @@ Steps through the whole iterator, counting the number of outputs emitted.
 
 This function's runtime is linear in the number of steps taken by the iterator.
 -/
-@[always_inline, inline]
+@[always_inline, inline, deprecated IterM.count (since := "2025-12-04")]
 def IterM.Partial.count {α : Type w} {m : Type w → Type w'} {β : Type w} [Iterator α m β]
-    [IteratorLoopPartial α m m] [Monad m] (it : IterM.Partial (α := α) m β) : m (ULift Nat) :=
-  it.fold (init := .up 0) fun acc _ => .up (acc.down + 1)
+    [IteratorLoop α m m] [Monad m] (it : IterM.Partial (α := α) m β) : m (ULift Nat) :=
+  it.it.fold (init := .up 0) fun acc _ => .up (acc.down + 1)
 
 /--
 Steps through the whole iterator, counting the number of outputs emitted.
@@ -661,8 +938,8 @@ This function's runtime is linear in the number of steps taken by the iterator.
 -/
 @[always_inline, inline, deprecated IterM.Partial.count (since := "2025-10-29")]
 def IterM.Partial.size {α : Type w} {m : Type w → Type w'} {β : Type w} [Iterator α m β]
-    [IteratorLoopPartial α m m] [Monad m] (it : IterM.Partial (α := α) m β) : m (ULift Nat) :=
-  it.count
+    [IteratorLoop α m m] [Monad m] (it : IterM.Partial (α := α) m β) : m (ULift Nat) :=
+  it.it.count
 
 end Count
 
