src/Init/Data/Iterators/Consumers/Monadic/Total.lean
@@ -1,0 +1,36 @@
+/-
+Copyright (c) 2025 Lean FRO, LLC. All rights reserved.
+Released under Apache 2.0 license as described in the file LICENSE.
+Authors: Paul Reichert
+-/
+module
+
+prelude
+public import Init.Data.Iterators.Basic
+
+set_option doc.verso true
+
+public section
+
+namespace Std.Iterators
+
+structure IterM.Total {α : Type w} (m : Type w → Type w') (β : Type w) where
+  it : IterM (α := α) m β
+
+/--
+For an iterator {name}`it`, {lean}`it.ensureTermination` provides variants of consumers that always
+terminate.
+-/
+@[always_inline, inline]
+def IterM.ensureTermination {α : Type w} {β : Type w} {m : Type w → Type w'}
+    (it : IterM (α := α) m β) :
+  IterM.Total (α := α) m β :=
+  ⟨it⟩
+
+/--
+A wrapper around an iterator that provides strictly terminating consumers. See
+{name}`IterM.ensureTermination`.
+-/
+add_decl_doc IterM.Total
+
+end Std.Iterators
