src/Init/Data/Iterators/Lemmas/Consumers/Monadic/Collect.lean
@@ -10,29 +10,49 @@ public import Init.Data.Array.Lemmas
 public import Init.Data.Iterators.Lemmas.Monadic.Basic
 public import Init.Data.Iterators.Consumers.Monadic.Collect
 import all Init.Data.Iterators.Consumers.Monadic.Collect
+import all Init.Data.Iterators.Consumers.Monadic.Total
+import all Init.WFExtrinsicFix
 
 public section
 
 namespace Std.Iterators
+open Std.Internal
 
 variable {α β γ : Type w} {m : Type w → Type w'} {n : Type w → Type w''}
   {lift : ⦃δ : Type w⦄ → m δ → n δ} {f : β → n γ} {it : IterM (α := α) m β}
 
-theorem IterM.DefaultConsumers.toArrayMapped.go.aux₁ [Monad n] [LawfulMonad n] [Iterator α m β]
-    [Finite α m] {b : γ} {bs : Array γ} :
+private theorem IterM.DefaultConsumers.toArrayMapped.go_eq [Monad n]
+    [Iterator α m β] [LawfulMonad n] [Finite α m] {acc : Array γ} :
+    letI : MonadLift m n := ⟨lift (δ := _)⟩
+    go lift f it acc (m := m) = (do
+      match (← it.step).inflate.val with
+      | .yield it' out => go lift f it' (acc.push (← f out))
+      | .skip it' => go lift f it' acc
+      | .done => return acc) := by
+  letI : MonadLift m n := ⟨lift (δ := _)⟩
+  rw [toArrayMapped.go, WellFounded.extrinsicFix₂_eq_apply]
+  · simp only
+    apply bind_congr; intro step
+    cases step.inflate using PlausibleIterStep.casesOn
+    · apply bind_congr; intro fx
+      simp [go]
+    · simp [go]
+    · simp
+  · simp only [show (IterM.finitelyManySteps! = IterM.finitelyManySteps) by rfl]
+    apply InvImage.wf
+    exact WellFoundedRelation.wf
+
+private theorem IterM.DefaultConsumers.toArrayMapped.go.aux₁ [Monad n] [LawfulMonad n]
+    [Iterator α m β] [Finite α m] {b : γ} {bs : Array γ} :
     IterM.DefaultConsumers.toArrayMapped.go lift f it (#[b] ++ bs) (m := m) =
       (#[b] ++ ·) <$> IterM.DefaultConsumers.toArrayMapped.go lift f it bs (m := m) := by
-  induction it, bs using IterM.DefaultConsumers.toArrayMapped.go.induct with | _ it bs ih₁ ih₂
-  rw [go, map_eq_pure_bind, go, bind_assoc]
-  apply bind_congr
-  intro step
-  split
-  · simp [ih₁ _ _ ‹_›]
-  · simp [ih₂ _ ‹_›]
-  · simp
+  induction it using IterM.inductSteps generalizing bs with | step it ihy ihs
+  rw [go_eq, map_eq_pure_bind, go_eq, bind_assoc]
+  apply bind_congr; intro step
+  cases step.inflate using PlausibleIterStep.casesOn <;> simp (discharger := assumption) [ihy, ihs]
 
-theorem IterM.DefaultConsumers.toArrayMapped.go.aux₂ [Monad n] [LawfulMonad n] [Iterator α m β]
-    [Finite α m] {acc : Array γ} :
+private theorem IterM.DefaultConsumers.toArrayMapped.go.aux₂ [Monad n] [LawfulMonad n]
+    [Iterator α m β] [Finite α m] {acc : Array γ} :
     IterM.DefaultConsumers.toArrayMapped.go lift f it acc (m := m) =
       (acc ++ ·) <$> IterM.DefaultConsumers.toArrayMapped lift f it (m := m) := by
   rw [← Array.toArray_toList (xs := acc)]
@@ -51,11 +71,17 @@ theorem IterM.DefaultConsumers.toArrayMapped_eq_match_step [Monad n] [LawfulMona
         return #[← f out] ++ (← IterM.DefaultConsumers.toArrayMapped lift f it' (m := m))
       | .skip it' => IterM.DefaultConsumers.toArrayMapped lift f it' (m := m)
       | .done => return #[]) := by
-  rw [IterM.DefaultConsumers.toArrayMapped, IterM.DefaultConsumers.toArrayMapped.go]
+  rw [IterM.DefaultConsumers.toArrayMapped, IterM.DefaultConsumers.toArrayMapped.go_eq]
   apply bind_congr
   intro step
   cases step.inflate using PlausibleIterStep.casesOn <;>
     simp [IterM.DefaultConsumers.toArrayMapped.go.aux₂]
+
+@[simp]
+theorem IterM.toArray_ensureTermination [Monad m] [Iterator α m β] [Finite α m]
+    [IteratorCollect α m m] {it : IterM (α := α) m β} :
+    it.ensureTermination.toArray = it.toArray :=
+  (rfl)
 
 theorem IterM.toArray_eq_match_step [Monad m] [LawfulMonad m] [Iterator α m β] [Finite α m]
     [IteratorCollect α m m] [LawfulIteratorCollect α m m] :
@@ -68,17 +94,42 @@ theorem IterM.toArray_eq_match_step [Monad m] [LawfulMonad m] [Iterator α m β]
   rw [IterM.DefaultConsumers.toArrayMapped_eq_match_step]
   simp [bind_pure_comp, pure_bind]
 
+theorem IterM.toArray_ensureTermination_eq_match_step [Monad m] [LawfulMonad m] [Iterator α m β]
+    [Finite α m] [IteratorCollect α m m] [LawfulIteratorCollect α m m] :
+    it.ensureTermination.toArray = (do
+      match (← it.step).inflate.val with
+      | .yield it' out => return #[out] ++ (← it'.toArray)
+      | .skip it' => it'.toArray
+      | .done => return #[]) := by
+  rw [toArray_ensureTermination, toArray_eq_match_step]
+
+@[simp]
+theorem IterM.toList_ensureTermination [Monad m] [Iterator α m β] [Finite α m]
+    [IteratorCollect α m m] {it : IterM (α := α) m β} :
+    it.ensureTermination.toList = it.toList :=
+  (rfl)
+
 @[simp]
 theorem IterM.toList_toArray [Monad m] [Iterator α m β] [Finite α m] [IteratorCollect α m m]
     {it : IterM (α := α) m β} :
     Array.toList <$> it.toArray = it.toList := by
   simp [IterM.toList]
 
+theorem IterM.toList_toArray_ensureTermination [Monad m] [Iterator α m β] [Finite α m]
+    [IteratorCollect α m m] {it : IterM (α := α) m β} :
+    Array.toList <$> it.ensureTermination.toArray = it.toList := by
+  simp
+
 @[simp]
 theorem IterM.toArray_toList [Monad m] [LawfulMonad m] [Iterator α m β] [Finite α m]
     [IteratorCollect α m m] {it : IterM (α := α) m β} :
     List.toArray <$> it.toList = it.toArray := by
   simp [IterM.toList, -toList_toArray]
+
+theorem IterM.toArray_toList_ensureTermination [Monad m] [LawfulMonad m] [Iterator α m β] [Finite α m]
+    [IteratorCollect α m m] {it : IterM (α := α) m β} :
+    List.toArray <$> it.ensureTermination.toList = it.toArray := by
+  rw [toList_ensureTermination, toArray_toList]
 
 theorem IterM.toList_eq_match_step [Monad m] [LawfulMonad m] [Iterator α m β] [Finite α m]
     [IteratorCollect α m m] [LawfulIteratorCollect α m m] {it : IterM (α := α) m β} :
@@ -93,17 +144,49 @@ theorem IterM.toList_eq_match_step [Monad m] [LawfulMonad m] [Iterator α m β] 
   intro step
   split <;> simp
 
-theorem IterM.toListRev.go.aux₁ [Monad m] [LawfulMonad m] [Iterator α m β] [Finite α m]
+theorem IterM.toList_ensureTermination_eq_match_step [Monad m] [LawfulMonad m] [Iterator α m β]
+    [Finite α m] [IteratorCollect α m m] [LawfulIteratorCollect α m m] {it : IterM (α := α) m β} :
+    it.ensureTermination.toList = (do
+      match (← it.step).inflate.val with
+      | .yield it' out => return out :: (← it'.toList)
+      | .skip it' => it'.toList
+      | .done => return []) := by
+  rw [toList_ensureTermination, toList_eq_match_step]
+
+@[simp]
+theorem IterM.toListRev_ensureTermination_eq_toListRev [Monad m] [Iterator α m β] [Finite α m]
+    {it : IterM (α := α) m β} :
+    it.ensureTermination.toListRev = it.toListRev :=
+  (rfl)
+
+private theorem IterM.toListRev.go_eq [Monad m] [LawfulMonad m] [Iterator α m β] [Finite α m]
+    {it : IterM (α := α) m β} {bs : List β} :
+    go it bs = (do
+      match (← it.step).inflate.val with
+      | .yield it' out => go it' (out :: bs)
+      | .skip it' => go it' bs
+      | .done => return bs) := by
+  rw [go, WellFounded.extrinsicFix₂_eq_apply]
+  · apply bind_congr; intro step
+    cases step.inflate using PlausibleIterStep.casesOn <;> simp [go]
+  · simp only [show (IterM.finitelyManySteps! = IterM.finitelyManySteps) by rfl]
+    apply InvImage.wf
+    exact WellFoundedRelation.wf
+
+private theorem IterM.toListRev.go.aux₁ [Monad m] [LawfulMonad m] [Iterator α m β] [Finite α m]
     {it : IterM (α := α) m β} {b : β} {bs : List β} :
     IterM.toListRev.go it (bs ++ [b]) = (· ++ [b]) <$> IterM.toListRev.go it bs:= by
-  induction it, bs using IterM.toListRev.go.induct with | _ it bs ih₁ ih₂
-  rw [go, go, map_eq_pure_bind, bind_assoc]
+  induction it using IterM.inductSteps generalizing bs with | step it ihy ihs
+  rw [go_eq, go_eq, map_eq_pure_bind, bind_assoc]
   apply bind_congr
   intro step
-  simp only [List.cons_append] at ih₁
-  split <;> simp [*]
+  cases step.inflate using PlausibleIterStep.casesOn
+  · simpa using ihy ‹_› (bs := _ :: bs)
+  · simpa using ihs ‹_›
+  · simp
 
-theorem IterM.toListRev.go.aux₂ [Monad m] [LawfulMonad m] [Iterator α m β] [Finite α m]
+
+private theorem IterM.toListRev.go.aux₂ [Monad m] [LawfulMonad m] [Iterator α m β] [Finite α m]
     {it : IterM (α := α) m β} {acc : List β} :
     IterM.toListRev.go it acc = (· ++ acc) <$> it.toListRev := by
   rw [← List.reverse_reverse (as := acc)]
@@ -120,11 +203,21 @@ theorem IterM.toListRev_eq_match_step [Monad m] [LawfulMonad m] [Iterator α m �
       | .skip it' => it'.toListRev
       | .done => return []) := by
   simp [IterM.toListRev]
-  rw [toListRev.go]
+  rw [toListRev.go_eq]
   apply bind_congr
   intro step
   cases step.inflate using PlausibleIterStep.casesOn <;> simp [IterM.toListRev.go.aux₂]
 
+theorem IterM.toListRev_ensureTermination_eq_match_step [Monad m] [LawfulMonad m] [Iterator α m β]
+    [Finite α m] {it : IterM (α := α) m β} :
+    it.ensureTermination.toListRev = (do
+      match (← it.step).inflate.val with
+      | .yield it' out => return (← it'.toListRev) ++ [out]
+      | .skip it' => it'.toListRev
+      | .done => return []) := by
+  rw [toListRev_ensureTermination_eq_toListRev, toListRev_eq_match_step]
+
+@[simp]
 theorem IterM.reverse_toListRev [Monad m] [LawfulMonad m] [Iterator α m β] [Finite α m]
     [IteratorCollect α m m] [LawfulIteratorCollect α m m]
     {it : IterM (α := α) m β} :
@@ -137,19 +230,31 @@ theorem IterM.reverse_toListRev [Monad m] [LawfulMonad m] [Iterator α m β] [Fi
   intro step
   cases step.inflate using PlausibleIterStep.casesOn <;> simp (discharger := assumption) [ihy, ihs]
 
+@[simp]
+theorem IterM.reverse_toListRev_ensureTermination [Monad m] [LawfulMonad m] [Iterator α m β]
+    [Finite α m] [IteratorCollect α m m] [LawfulIteratorCollect α m m]
+    {it : IterM (α := α) m β} :
+    List.reverse <$> it.ensureTermination.toListRev = it.toList := by
+  rw [toListRev_ensureTermination_eq_toListRev, reverse_toListRev]
+
 theorem IterM.toListRev_eq [Monad m] [LawfulMonad m] [Iterator α m β] [Finite α m]
     [IteratorCollect α m m] [LawfulIteratorCollect α m m]
     {it : IterM (α := α) m β} :
     it.toListRev = List.reverse <$> it.toList := by
-  rw [← IterM.reverse_toListRev]
-  simp
+  simp [← IterM.reverse_toListRev]
+
+theorem IterM.toListRev_ensureTermination [Monad m] [LawfulMonad m] [Iterator α m β] [Finite α m]
+    [IteratorCollect α m m] [LawfulIteratorCollect α m m]
+    {it : IterM (α := α) m β} :
+    it.ensureTermination.toListRev = List.reverse <$> it.toList := by
+  simp [← IterM.reverse_toListRev]
 
 theorem LawfulIteratorCollect.toArray_eq {α β : Type w} {m : Type w → Type w'}
     [Monad m] [Iterator α m β] [Finite α m] [IteratorCollect α m m]
     [hl : LawfulIteratorCollect α m m]
     {it : IterM (α := α) m β} :
     it.toArray = (letI : IteratorCollect α m m := .defaultImplementation; it.toArray) := by
-  simp only [IterM.toArray, toArrayMapped_eq]
+  simp [IterM.toArray, toArrayMapped_eq, IteratorCollect.defaultImplementation]
 
 theorem LawfulIteratorCollect.toList_eq {α β : Type w} {m : Type w → Type w'}
     [Monad m] [Iterator α m β] [Finite α m] [IteratorCollect α m m]
